Cleanup.

proof/garbleTools.ec
@@ -16,60 +16,63 @@ type 'a gate = 'a*'a*'a*'a.
 type fGate = bool gate.
 type gGate = token gate.
 
-op getTok(x:tokens, a:int, i:bool) : token =
+op getTok (x:tokens) (a:int) (i:bool): token =
   if i then snd x.[a] else fst x.[a].
 
-op setTok(x:tokens, a:int, i:bool, t:token) : tokens =
+op setTok (x:tokens) (a:int) (i:bool) (t:token): tokens =
   if i then x.[a <- (fst x.[a], t)] else x.[a <- (t, snd x.[a])].
 
-lemma set_get_tok: forall (x:tokens, a:int, i:bool, t:token, b:int, j:bool),
-  0 <= b => b < length x =>
-  getTok (setTok x a i t) b j = (a=b/\i=j)?t:getTok x b j.
-intros=> ? ? ? ? ? ? ? ?.
-simplify setTok getTok.
-by case i=> ?;case j=> ?;rewrite ! set_get //;case (a=b)=> ?;subst;trivial.
+lemma set_get_tok (x:tokens) (a:int) (i:bool) (t:token) (b:int) (j:bool):
+  0 <= b < length x =>
+  getTok (setTok x a i t) b j =
+    if (a = b /\ i = j) then t else getTok x b j.
+proof strict.
+by intros=> [leq0_b ltb_lenx]; rewrite /setTok /getTok /=;
+   case i; case j; rewrite !set_get //; case (a = b).
 qed.
 
-lemma set_set_tok: forall (x:tokens, a:int, i:bool, t:token, u:token),
-  0 <= a => a < Array.length x =>
+lemma set_set_tok (x:tokens) (a:int) (i:bool) (t:token) (u:token):
+  0 <= a < Array.length x =>
   setTok (setTok x a i t) a i u = (setTok x a i u).
-  intros=> ? ? ? ? ? ? ?.
-  simplify setTok fst snd.
-  case i=> ?;simplify;rewrite set_setE  set_get //. 
+proof strict.
+by intros=> [leq0_a lta_lenx]; rewrite /setTok /setTok /fst /snd /=;
+   case i; rewrite set_setE set_get.
 qed.
 
-lemma nosmt set_tokC: forall (x:tokens, a:int, i:bool, b:int, j:bool, t:token, u:token),
-  0 <= a < Array.length x => 0 <= b < Array.length x => a <> b \/ i <> j =>
+lemma nosmt set_tokC (x:tokens) (a:int) (i:bool) (b:int) (j:bool) (t:token) (u:token):
+  0 <= a < Array.length x =>
+  0 <= b < Array.length x =>
+  a <> b \/ i <> j =>
   setTok (setTok x a i t) b j u = setTok (setTok x b j u) a i t
-  by (progress;simplify setTok;apply extensionality;(split;last case i=> ?);smt).
+by (progress;simplify setTok;apply extensionality;(split;last case i);smt).
 
-lemma length_setTok: forall (x:tokens, a:int, i:bool, t:token),
+lemma length_setTok (x:tokens) (a:int) (i:bool) (t:token):
   length (setTok x a i t) = length x
-  by smt.
+by [].
 
 op intToBitstring = zeros.
 
-lemma intToBitstring_inj : forall g gg,
-0 <= g => 0 <= gg =>
-intToBitstring g = intToBitstring gg =>
-g = gg.
-intros=> ? ? ? ?.
-rewrite /intToBitstring -Bits.rw_ext /Bits.(==)! zeros_length //.
+lemma intToBitstring_inj g g':
+  0 <= g => 0 <= g' =>
+  intToBitstring g = intToBitstring g' =>
+  g = g'.
+proof strict.
+by intros=> leq0_g leq0_g';
+   rewrite /intToBitstring -Bits.rw_ext /Bits.(==) !zeros_length.
 qed.
 
-op tweak(g:int, a:bool, b:bool) : bitstring = a::(b::(intToBitstring g)).
+op tweak (g:int) (a:bool) (b:bool): bitstring = a::(b::(intToBitstring g)).
 
-lemma tweak_inj :
-  forall g a b gg aa bb, 0 <= g => 0 <= gg =>
-     tweak g a b = tweak gg aa bb => (g, a, b) = (gg, aa, bb).
-intros ? ? ? ? ? ? ? ?.
-simplify tweak.
-rewrite ! Bits.cons_inj=> [? [? ?]].
-subst;split=> //.
-apply intToBitstring_inj=> //.
+lemma tweak_inj g a b g' a' b':
+  0 <= g => 0 <= g' =>
+  tweak g a b = tweak g' a' b' =>
+  (g, a, b) = (g', a', b').
+proof strict.
+by intros=> leq0_g leq0_g'; rewrite /tweak !Bits.cons_inj=> [<- [<- eqGb]];
+   split=> //; apply intToBitstring_inj.
 qed.
 
-op evalGate(f:'a gate, i:bool*bool) : 'a =
+op evalGate (f:'a gate) (i:bool * bool): 'a =
   let (ff, ft, tf, tt) = f in
   let (i1, i2) = i in
   if !i1 && !i2 then ff else
@@ -77,7 +80,7 @@ op evalGate(f:'a gate, i:bool*bool) : 'a =
   if  i1 && !i2 then tf else
   tt.
 
-op setGateVal(f:'a gate, i:bool*bool, v:'a) : 'a gate =
+op setGateVal (f:'a gate) (i:bool*bool) (v:'a) : 'a gate =
   let (ff, ft, tf, tt) = f in
   let (i1, i2) = i in
   if !i1 && !i2 then ( v, ft, tf, tt) else
@@ -85,14 +88,14 @@ op setGateVal(f:'a gate, i:bool*bool, v:'a) : 'a gate =
   if  i1 && !i2 then (ff, ft,  v, tt) else
   (ff, ft, tf,  v).
 
-pred tokenCorrect(n:int, q:int, m:int, x:tokens) =
-  Array.length x = (n+q) /\
-  (forall (i:int), 0 <= i => i < n + q =>
-    (DKC.lsb (getTok x i false)) <> (DKC.lsb (getTok x i true))) /\
-  (forall (i:int), n + q - m <= i => i < n + q =>
-    !(DKC.lsb (getTok x i false)) ).
+pred tokenCorrect (n:int) (q:int) (m:int) (x:tokens) =
+  Array.length x = n + q /\
+  (forall (i:int), 0 <= i < n + q =>
+    DKC.lsb (getTok x i false) <> DKC.lsb (getTok x i true)) /\
+  (forall (i:int), n + q - m <= i < n + q =>
+    !DKC.lsb (getTok x i false)).
 
-op enc(x:tokens, f:fGate, a:int, b:int, g:int, x1:bool, x2:bool) : token =
+op enc (x:tokens) (f:fGate) (a:int) (b:int) (g:int) (x1:bool) (x2:bool): token =
   let xx1 = (DKC.lsb (getTok x a true) = x1) in
   let xx2 = (DKC.lsb (getTok x b true) = x2) in
   DKC.E
@@ -101,50 +104,40 @@ op enc(x:tokens, f:fGate, a:int, b:int, g:int, x1:bool, x2:bool) : token =
     (getTok x b xx2)
     (getTok x g (evalGate f (xx1,xx2))).
 
-
-op garbleGate(x:tokens, f:fGate, a:int, b:int, g:int) : gGate =
-  (
-    enc x f a b g false false,
+op garbleGate (x:tokens) (f:fGate) (a:int) (b:int) (g:int) : gGate =
+  ( enc x f a b g false false,
     enc x f a b g false  true,
     enc x f a b g  true false,
-    enc x f a b g  true  true
-  ).
+    enc x f a b g  true  true ).
 
-lemma inverse_base :
-    (forall (t k1 k2 m:Dkc.t), DKC.D t k1 k2 (DKC.E t k1 k2 m) = m) =>
-    forall (i1 i2: bool) ,
-    forall (n q m a b g : int) ,
-    forall (f : fGate) ,
-    forall (x : tokens) ,
-      (n > 0) =>
-      (q > 0) =>
-      (m > 0) =>
-      (0 <= a) /\ (a < g) =>
-      (0 <= b) /\ (b < g) =>
-      (n <= g /\ g < n + q) =>
-      tokenCorrect n q m x =>
-      DKC.D
-        (tweak g (DKC.lsb (getTok x a i1)) (DKC.lsb (getTok x b i2))) (getTok x a i1) (getTok x b i2)
-        (evalGate
-          (garbleGate x f a b g)
-          (DKC.lsb (getTok x a i1), DKC.lsb (getTok x b i2))
-        ) = getTok x g (evalGate f (i1, i2)).
+lemma inverse_base i1 i2 n q m a b g f x:
+  (forall (t k1 k2 m:Dkc.t), DKC.D t k1 k2 (DKC.E t k1 k2 m) = m) =>
+  0 < n =>
+  0 < q =>
+  0 < m =>
+  0 <= a < g =>
+  0 <= b < g =>
+  n <= g < n + q =>
+  tokenCorrect n q m x =>
+  DKC.D
+    (tweak g (DKC.lsb (getTok x a i1)) (DKC.lsb (getTok x b i2))) (getTok x a i1) (getTok x b i2)
+    (evalGate
+      (garbleGate x f a b g)
+      (DKC.lsb (getTok x a i1), DKC.lsb (getTok x b i2))
+    ) = getTok x g (evalGate f (i1, i2)).
 proof strict.
-  intros DKCinv.
-  do intros ?.
-  pose gi1 := (getTok x a i1).
-  pose gi2 := (getTok x b i2).
-  rewrite -(DKCinv (tweak g (DKC.lsb gi1) (DKC.lsb gi2)) gi1 gi2 (getTok x g (evalGate f (i1, i2)))).
-  congr=> //. 
-  simplify evalGate garbleGate enc.
-  generalize H5.
-  case (! DKC.lsb gi1 && ! DKC.lsb gi2)=> h;smt.
+intros=> DKCCor lt0_n lt0_q lt0_m
+         [leq0_a lta_g] [leq0_b ltb_g]
+         [leqn_g ltg_nb] tCor.
+pose gi1:= (getTok x a i1); pose gi2:= (getTok x b i2).
+rewrite -(DKCCor (tweak g (DKC.lsb gi1) (DKC.lsb gi2)) gi1 gi2 (getTok x g (evalGate f (i1, i2)))).
+congr=> //; rewrite /evalGate /garbleGate /enc.
+by case (!DKC.lsb gi1 && !DKC.lsb gi2)=> h; smt.
 qed.
 
-
 type w2g = int array.
-type 'a g2v = ('a*'a*'a*'a) array.
-type 'a functGen = int*int*int*w2g*w2g*('a g2v).
+type 'a g2v = ('a * 'a * 'a * 'a) array.
+type 'a functGen = int * int * int * w2g * w2g * ('a g2v).
 
 (*Access to funct member*)
 op getN(f:'a functGen) : int =
@@ -160,20 +153,19 @@ op getB(f:'a' functGen) : w2g =
 op getG(f:'a functGen) : 'a g2v =
   let (n, m, q, a, b, g) = f in g.
 
-op evalComplete(f:'a functGen, x:'a array, extract:'a functGen -> int -> 'a array -> 'a) : 'a array =
+op evalComplete (f:'a functGen) (x:'a array) (extract:'a functGen -> int -> 'a array -> 'a): 'a array =
   appendInit x (getQ f) (extract f).
 
-op evalGen(f:'a functGen, x:'a array, extract:'a functGen -> int -> 'a array -> 'a) : 'a array =
-  Array.sub (evalComplete f x extract) ((getN f) + (getQ f) - (getM f)) (getM f).
+op evalGen (f:'a functGen) (x:'a array) (extract:'a functGen -> int -> 'a array -> 'a): 'a array =
+  Array.sub (evalComplete f x extract) (getN f + getQ f - getM f) (getM f).
 
-op extract(f:bool functGen, g:int, x:bool array) : bool =
+op extract (f:bool functGen) (g:int) (x:bool array): bool =
   let g = g + 1 in
   evalGate (getG f).[g] (x.[(getA f).[g]], x.[(getB f).[g]]).
 
-
-op eval(f:bool functGen, i:bool array, k:int) = (evalComplete f i extract).[k].
+op eval (f:bool functGen) (i:bool array) (k:int) = (evalComplete f i extract).[k].
   
-op extractG(ff:token functGen, g:int, x:token array) =
+op extractG (ff:token functGen) (g:int) (x:token array) =
   let g = g + 1 in
   let a = (getA ff).[g] in
   let b = (getB ff).[g] in
@@ -184,62 +176,51 @@ op extractG(ff:token functGen, g:int, x:token array) =
   let t = tweak g a b in
   DKC.D t aA bB (evalGate ((getG ff).[g]) (a, b)).
 
-
-op garbMap(x:tokens, f:bool functGen, g:int) : token*token*token*token =
+op garbMap (x:tokens) (f:bool functGen) (g:int): token * token * token * token =
   garbleGate x (getG f).[g] (getA f).[g] (getB f).[g] g.
 
-op choose(k:(token*token) array, i:bool array, j:int) : token = getTok k j i.[j].
+op choose (k:(token*token) array) (i:bool array) (j:int): token = getTok k j i.[j].
 
-op validCircuit(bound:int, f:(bool functGen)) =
+op validCircuit (bound:int) (f:bool functGen) =
   let (n, m, q, aa, bb, gg) = f in
-  n > 1 /\ m > 0 /\ q > 0 /\ q >= m /\
+  1 < n /\ 0 < m /\ 0 < q /\ m <= q /\
   n + q - m = bound /\
   length aa = n + q /\ length bb = n + q /\ length gg = n + q /\
-  (range n (n+q) true (lambda i b, b /\ aa.[i] >= 0 /\ bb.[i] < i /\ bb.[i] < n+q-m /\ aa.[i] < bb.[i])).
+  (range n (n + q) true (lambda i b, b /\ 0 <= aa.[i] /\ bb.[i] < i /\ bb.[i] < n+q-m /\ aa.[i] < bb.[i])).
 
-lemma valid_wireinput :
-  forall (bound:int) (f:(bool functGen)),
-    validCircuit bound f <=> 
+lemma valid_wireinput (bound:int) (f:bool functGen):
+  validCircuit bound f <=> 
   let (n, m, q, aa, bb, gg) = f in
-  n > 1 /\ m > 0 /\ q > 0 /\ q >= m /\
+  1 < n /\ 0 < m /\ 0 < q /\ m <= q /\
   n + q - m = bound /\
   Array.length aa = n + q /\ Array.length bb = n + q /\ Array.length gg = n + q /\
       (forall i,
-         i >= n  => i < n+q =>
-           aa.[i] >= 0 /\
+         n <= i < n+q =>
+           0 <= aa.[i] /\
            bb.[i] < i /\
            bb.[i] < n+q-m /\
            aa.[i] < bb.[i]).
-delta validCircuit.
-intros bound f.
-elim/tuple6_ind f.
-intros n m q aa bb gg valF.
-case (n > 1);last simplify;smt.
-case (m > 0);last simplify;split.
-case (q > 0);last simplify;split.
-case (n + q - m = bound);last simplify;split.
-case (length aa = n + q);last simplify;split.
-case (length bb = n + q);last simplify;split.
-case (length gg = n + q);last simplify;split.
-intros H1 H2 H3 H4 H5 H6 H7.
-rewrite (_:(n > 1) = true);first smt.
-simplify.
-apply (_:forall a b d, (b <=> d) => (a /\ b <=> a /\ d));first smt.
+proof strict.
+rewrite /validCircuit; elim/tuple6_ind f=> n m q aa bb gg valF.
+case (1 < n); last smt. (* EC Note: Different behaviour between first member of a conjunction and others in goal? *)
+case (0 < m)=> //.
+case (0 < q)=> //.
+case (n + q - m = bound)=> //.
+case (length aa = n + q)=> //.
+case (length bb = n + q)=> //.
+case (length gg = n + q)=> //.
+intros=> H1 H2 H3 H4 H5 H6 -> /=.
+apply (_: forall b d, (b <=> d) => (m <= q /\ b <=> m <= q /\ d)); first smt.
 pose {1 3} j := q.
-elim/Induction.induction j;last first;first 2 smt.
-simplify => k hypJ hypRec.
-rewrite range_ind;first smt.
-rewrite (_:(n + (k+1) - 1 = n + k));first smt.
-rewrite hypRec.
-simplify.
-split => h.
-elim h => h1 h2 i.
+elim/Induction.induction j; last first; first 2 smt.
+intros=> k hypJ hypRec.
+rewrite range_ind; first smt.
+rewrite (_: n + (k + 1) - 1 = n + k); first smt.
+rewrite hypRec /=.
+split=> h.
+elim h=> h1 h2 i.
 case (i = n + k).
-  intros => -> _ _.
-apply h2.
-intros hh1 hh2 hh3.
-apply h1.
-assumption.
-smt.
-(split;first intros i hI hI2);apply h;smt.
+  by intros => -> _; apply h2.
+  by intros=> hh1 hh2; smt.
+(split;first intros i hI);apply h;smt.
 qed.
